notes/04-lecture-07.v
@@ -1,0 +1,159 @@
+(*
+
+If you have programs that don't terminate,
+
+an _interpreter_ will not be able to prove all of its semantics.
+
+Instead, we can use _transisition systems_.
+
+*)
+
+(********************** Begin: FRAP Preamble **********************)
+Require Import Frap.
+
+Set Implicit Arguments.
+
+Fixpoint fact (n : nat) : nat :=
+  match n with
+  | O => 1
+  | S n' => fact n' * S n'
+  end.
+
+Inductive fact_state :=
+| AnswerIs (answer : nat)
+| WithAccumulator (input accumulator : nat).
+
+Inductive fact_init (original_input : nat) : fact_state -> Prop :=
+| FactInit : fact_init original_input (WithAccumulator original_input 1).
+
+Inductive fact_final : fact_state -> Prop :=
+| FactFinal : forall ans, fact_final (AnswerIs ans).
+
+Inductive fact_step : fact_state -> fact_state -> Prop :=
+| FactDone : forall acc,
+  fact_step (WithAccumulator O acc) (AnswerIs acc)
+| FactStep : forall n acc,
+  fact_step (WithAccumulator (S n) acc) (WithAccumulator n (acc * S n)).
+
+Inductive trc {A} (R : A -> A -> Prop) : A -> A -> Prop :=
+| TrcRefl : forall x, trc R x x
+| TrcFront : forall x y z,
+  R x y
+  -> trc R y z
+  -> trc R x z.
+
+Set Warnings "-notation-overridden".
+Notation "R ^*" := (trc R) (at level 0).
+
+Example factorial_3 : fact_step^* (WithAccumulator 3 1) (AnswerIs 6).
+Proof.
+Admitted.
+
+Record trsys state := {
+  Initial : state -> Prop;
+  Step : state -> state -> Prop
+}.
+
+Definition factorial_sys (original_input : nat) : trsys fact_state := {|
+  Initial := fact_init original_input;
+  Step := fact_step
+|}.
+
+Inductive reachable {state} (sys : trsys state) (st : state) : Prop :=
+| Reachable : forall st0,
+  sys.(Initial) st0
+  -> sys.(Step)^* st0 st
+  -> reachable sys st.
+(********************** End: FRAP Preamble **********************)
+
+(*
+Q: why is sys.(Initial) s necessary in `forall s, sys.(Initial) s` ?
+A: look at its definition, this means `forall s that is an initial state of sys`
+   so altogether, this is the statement:
+   "forall initial states s of sys,
+     forall states s' reachable from s,
+      invariant holds for s'"
+*)
+Definition invariantFor {state} (sys : trsys state) (invariant : state -> Prop) :=
+  forall s, sys.(Initial) s
+            -> forall s', sys.(Step)^* s s'
+                          -> invariant s'.
+
+(********************** Begin: FRAP Preamble **********************)
+Lemma use_invariant' : forall {state} (sys : trsys state)
+  (invariant : state -> Prop) s s',
+  invariantFor sys invariant
+  -> sys.(Initial) s
+  -> sys.(Step)^* s s'
+  -> invariant s'.
+Proof.
+  unfold invariantFor.
+  simplify.
+  eapply H.
+  eassumption.
+  assumption.
+Qed.
+
+Theorem use_invariant : forall {state} (sys : trsys state)
+  (invariant : state -> Prop) s,
+  invariantFor sys invariant
+  -> reachable sys s
+  -> invariant s.
+Proof.
+  simplify.
+  invert H0.
+  eapply use_invariant'.
+  eassumption.
+  eassumption.
+  assumption.
+Qed.
+
+Lemma invariant_induction' : forall {state} (sys : trsys state)
+  (invariant : state -> Prop),
+  (forall s, invariant s -> forall s', sys.(Step) s s' -> invariant s')
+  -> forall s s', sys.(Step)^* s s'
+     -> invariant s
+     -> invariant s'.
+Proof.
+  induct 2; propositional.
+  apply IHtrc.
+  eapply H.
+  eassumption.
+  assumption.
+Qed.
+
+Theorem invariant_induction : forall {state} (sys : trsys state)
+  (invariant : state -> Prop),
+  (forall s, sys.(Initial) s -> invariant s)
+  -> (forall s, invariant s -> forall s', sys.(Step) s s' -> invariant s')
+  -> invariantFor sys invariant.
+Proof.
+  unfold invariantFor; intros.
+  eapply invariant_induction'.
+  eassumption.
+  eassumption.
+  apply H.
+  assumption.
+Qed.
+
+Definition fact_invariant (original_input : nat) (st : fact_state) : Prop :=
+  match st with
+  | AnswerIs n => fact original_input = n
+  | WithAccumulator n acc => fact original_input = acc * fact n
+  end.
+(********************** End: FRAP Preamble **********************)
+
+(*
+Invert is very similar to cases or destruct, but it is smarter
+in that it can look backwards, looking at constraints in the type signature:
+
+"s is Initial => s was made with fact_init => s looks like WithAccumulator"
+*)
+Theorem fact_invariant_ok : forall original_input,
+  invariantFor (factorial_sys original_input) (fact_invariant original_input).
+Proof.
+  intros.
+  apply invariant_induction; simplify.
+  - invert H. simplify. auto.
+  - invert H0; simplify; linear_arithmetic.
+Qed.
