notes/frap-05-transition-systems.v
@@ -1,0 +1,273 @@
+(*
+Notes compiled from Studio Episode 5, Lectures 6-7
+Template from FRAP Ch 5: Transition Systems
+*)
+Require Import Frap.
+
+Set Implicit Arguments.
+
+Fixpoint fact (n : nat) : nat :=
+  match n with
+  | O => 1
+  | S n' => fact n' * S n'
+  end.
+
+Inductive fact_state :=
+| AnswerIs (answer : nat)
+| WithAccumulator (input accumulator : nat).
+
+Inductive fact_init (original_input : nat) : fact_state -> Prop :=
+| FactInit : fact_init original_input (WithAccumulator original_input 1).
+
+Check fact_init. (* fact_init : nat -> fact_state -> Prop *)
+(* so fact_init is a type constructor that takes a natural number, a
+*  fact_state, and produces a type whose type is Prop *)
+
+(* Notice the args to a type constructor before the initial colon
+*  (original_input above) are automatically arguments to each of
+*  the inductive constructors *)
+
+Check (fact_init 2 (AnswerIs 5)).
+(* Produces a type whose type is Prop. Happens to be false! *)
+
+Lemma fool :
+  fact_init 3 (WithAccumulator 3 1).
+Proof.
+  Show Proof.
+  exact (FactInit 3).
+  Restart.
+  constructor. (* or find the right constructor automatically *)
+  Show Proof.
+Qed.
+
+Lemma foo2 :
+  not (fact_init 5 (WithAccumulator 3 1)).
+Proof.
+  Print not.
+  unfold not.
+  intros.
+  invert H. (* find the only way we could have made H, via FactInit *)
+Qed.
+
+(*
+*  thought: why doesn't Coq just restrict type system so that we can only construct
+*           fact_inits via the FactInit constructor?
+*
+*  ben: we want a language that's strong enough to encode false statements
+*)
+
+Inductive fact_final : fact_state -> Prop :=
+| FactFinal : forall ans, fact_final (AnswerIs ans).
+
+(* Compare fact_step ... *)
+
+Inductive fact_step : fact_state -> fact_state -> Prop :=
+| FactDone : forall acc,
+  fact_step (WithAccumulator O acc) (AnswerIs acc)
+| FactStep : forall n acc,
+  fact_step (WithAccumulator (S n) acc) (WithAccumulator n (acc * S n)).
+
+(* to a more typical definition ... *)
+
+Definition plus : nat -> nat -> nat :=
+  (* the actual defn *)
+  fun a => fun b => a + b.
+
+(*
+Notice fact_step doesn't read as directly. It's a type that takes two values
+and produces a type whose type is Prop.
+
+But the only way to construct _values_ that inhibit the type `fact_step s1 s2`
+are via the `FactDone` and `FactStep` constructors.
+
+Also, fact_step, FactDone, FactStep are fundamentally different than plus. When
+we apply values to the former constructors, we don't compute and return values.
+Essentially all that happens when we apply values to the former is that we tag
+certain values to have certain types.
+*)
+
+Inductive trc {A} (R : A -> A -> Prop) : A -> A -> Prop :=
+| TrcRefl : forall x, trc R x x
+| TrcFront : forall x y z,
+  R x y
+  -> trc R y z
+  -> trc R x z.
+Set Warnings "-notation-overridden".
+Notation "R ^*" := (trc R) (at level 0).
+
+(* Now let's use it to execute the factorial program. *)
+Example factorial_3' : fact_step^* (WithAccumulator 3 1) (AnswerIs 6).
+Proof.
+  try constructor. (* fails with "unable to find instance for variable y" *)
+  econstructor. (* pretend y exists for a minute *)
+  constructor.
+  econstructor.
+  constructor.
+  econstructor.
+  constructor.
+  econstructor.
+  constructor.
+  simplify.
+  constructor. (* TrcRefl *)
+Qed.
+
+(* Or more succinctly: *)
+Example factorial_3 : fact_step^* (WithAccumulator 3 1) (AnswerIs 6).
+Proof.
+  (* repeat can be used to continue trying something until it stops making progress *)
+  (* repeat (let x := fresh in assert (x : True) by auto). makes infinite loop! *)
+  repeat (econstructor).
+Qed.
+
+(* If you have programs that don't terminate,
+   an _interpreter_ will not be able to prove all of its semantics.
+   Instead, we can use _transisition systems_.  *)
+Record trsys state := {
+  Initial : state -> Prop;
+  Step : state -> state -> Prop
+}.
+
+Definition factorial_sys (original_input : nat) : trsys fact_state := {|
+  Initial := fact_init original_input;
+  Step := fact_step
+|}.
+
+(* the {type} curly braces mean the type can be implicit and inferred by type
+*  checker.
+*
+*  to pass in {type} manually, prefix the function by '@'.
+*)
+
+Inductive reachable {state} (sys : trsys state) (st : state) : Prop :=
+| Reachable : forall st0,
+  sys.(Initial) st0
+  -> sys.(Step)^* st0 st
+  -> reachable sys st.
+(*
+Even though we use `forall`, we read as `exists`.
+*)
+Print ex.
+(*
+Inductive ex (A : Type) (P : A -> Prop) : Prop :=
+    ex_intro : forall x : A, P x -> exists y, P y
+
+So to build a _value_ of this type, we pass in _any_ x to ex_intro,
+such that P x is true.
+
+This is just because this is how constructors work, they take _any_ values that
+their type implies. By also requiring P x, the ability to call ex_intro (P x),
+we have shown that such an x does exist!
+*)
+
+Lemma foo :
+  exists n, n = S O.
+Proof.
+  exists 1; auto.
+Qed.
+
+Definition invariantFor {state} (sys : trsys state) (invariant : state -> Prop) :=
+  forall s, sys.(Initial) s
+            -> forall s', sys.(Step)^* s s'
+                          -> invariant s'.
+(*
+Q: above, why is sys.(Initial) s necessary in `forall s, sys.(Initial) s` ?
+A: look at its definition, this means `forall s that is an initial state of sys`
+   so altogether, this is the statement:
+   "forall initial states s of sys,
+     forall states s' reachable from s,
+      invariant holds for s'"
+*)
+
+(* for example, trivially, reachability is an invariant ! *)
+Lemma bar :
+  forall {state} (sys: trsys state),
+    invariantFor sys (reachable sys).
+Proof.
+  intros.
+  unfold invariantFor.
+  intros.
+  (* Notice H and H0 are precisely the arguments of the Reachable constructor
+     to create the `reachable sys s'` goal!  *)
+  econstructor; eauto.
+Qed.
+
+Lemma use_invariant' : forall {state} (sys : trsys state)
+  (invariant : state -> Prop) s s',
+  invariantFor sys invariant
+  -> sys.(Initial) s
+  -> sys.(Step)^* s s'
+  -> invariant s'.
+Proof.
+  unfold invariantFor.
+  simplify.
+  eapply H.
+  eassumption.
+  assumption.
+Qed.
+
+Theorem use_invariant : forall {state} (sys : trsys state)
+  (invariant : state -> Prop) s,
+  invariantFor sys invariant
+  -> reachable sys s
+  -> invariant s.
+Proof.
+  simplify.
+  invert H0.
+  eapply use_invariant'.
+  eassumption.
+  eassumption.
+  assumption.
+Qed.
+
+Lemma invariant_induction' : forall {state} (sys : trsys state)
+  (invariant : state -> Prop),
+  (forall s, invariant s -> forall s', sys.(Step) s s' -> invariant s')
+  -> forall s s', sys.(Step)^* s s'
+     -> invariant s
+     -> invariant s'.
+Proof.
+  (* induct 2 inducts on the second inductively defined datatype in the statement,
+     in this case:  sys.(Step)^* s s'
+   *)
+  induct 2; propositional.
+  apply IHtrc.
+  eapply H; eauto.
+  (* Many times this well let Coq find the right arg to H.
+     If it doesn't work, we can manually specify, but it might have been better
+     to just use apply (H x) in the first place. *)
+Qed.
+
+Theorem invariant_induction : forall {state} (sys : trsys state)
+  (invariant : state -> Prop),
+  (forall s, sys.(Initial) s -> invariant s)
+  -> (forall s, invariant s -> forall s', sys.(Step) s s' -> invariant s')
+  -> invariantFor sys invariant.
+Proof.
+  unfold invariantFor; intros.
+  eapply invariant_induction'.
+  eassumption.
+  eassumption.
+  apply H.
+  assumption.
+Qed.
+
+Definition fact_invariant (original_input : nat) (st : fact_state) : Prop :=
+  match st with
+  | AnswerIs n => fact original_input = n
+  | WithAccumulator n acc => fact original_input = acc * fact n
+  end.
+
+(*
+Invert is very similar to cases or destruct, but it is smarter
+in that it can look backwards, looking at constraints in the type signature:
+
+"s is Initial => s was made with fact_init => s looks like WithAccumulator"
+*)
+Theorem fact_invariant_ok : forall original_input,
+  invariantFor (factorial_sys original_input) (fact_invariant original_input).
+Proof.
+  intros.
+  apply invariant_induction; simplify.
+  - invert H. simplify. auto.
+  - invert H0; simplify; linear_arithmetic.
+Qed.
