notes/README.md
@@ -1,0 +1,8 @@
+# notes
+
+Files of the form `n-medium-m.v` are notes taken during the `n`th week and
+`m`th `medium`, e.g. `03-studio-05.v` contains notes from Studio Episode 5
+released during week 3. Some of these files contain redundant content since we
+go over the same chapters multiple times. Files prefixed with `frap-` contain
+the compiled notes for a given FRAP chapter, fighting redundancy with
+redundancy.
